hax-lib/proof-libs/fstar/rust_primitives/Rust_primitives.Arithmetic.fsti
@@ -3,6 +3,9 @@ module Rust_primitives.Arithmetic
 open FStar.Mul
 open Rust_primitives.Integers
 
+let rec int_pow (x: int) (n: nat) : Tot int (decreases n) =
+  if n = 0 then 1 else x * int_pow x (n - 1)
+
 let wrapping_add_u8 : u8 -> u8 -> u8 = add_mod
 let saturating_add_u8 : u8 -> u8 -> u8 = add_sat
 let overflowing_add_u8 : u8 -> u8 -> u8 & bool = add_overflow
@@ -18,7 +21,7 @@ val saturating_mul_u8 : u8 -> u8 -> u8
 let overflowing_mul_u8 : u8 -> u8 -> u8 & bool = mul_overflow
 let rem_euclid_u8 (x: u8) (y: u8 {v y <> 0}): u8 = x %! y
 val pow_u8 : u8 -> u32 -> u8
-val overflowing_pow_u8 : u8 -> u32 -> u8 & bool
+val overflowing_pow_u8 : x:u8 -> y:u32 -> r:(u8 & bool) {snd r == not (range (int_pow (v x) (v y)) U8)}
 val count_ones_u8 : u8 -> r:u32{v r <= 8}
 
 let wrapping_add_u16 : u16 -> u16 -> u16 = add_mod
@@ -36,7 +39,7 @@ val saturating_mul_u16 : u16 -> u16 -> u16
 let overflowing_mul_u16 : u16 -> u16 -> u16 & bool = mul_overflow
 let rem_euclid_u16 (x: u16) (y: u16 {v y <> 0}): u16 = x %! y
 val pow_u16 : x:u16 -> y:u32 -> result : u16 {v x == 2 /\ v y < 16 ==> result == mk_u16 (pow2 (v y))}
-val overflowing_pow_u16 : u16 -> u32 -> u16 & bool
+val overflowing_pow_u16 : x:u16 -> y:u32 -> r:(u16 & bool) {snd r == not (range (int_pow (v x) (v y)) U16)}
 val count_ones_u16 : u16 -> r:u32{v r <= 16}
 
 let wrapping_add_u32 : u32 -> u32 -> u32 = add_mod
@@ -54,7 +57,7 @@ val saturating_mul_u32 : u32 -> u32 -> u32
 let overflowing_mul_u32 : u32 -> u32 -> u32 & bool = mul_overflow
 let rem_euclid_u32 (x: u32) (y: u32 {v y <> 0}): u32 = x %! y
 val pow_u32 : x:u32 -> y:u32 -> result : u32 {v x == 2 /\ v y <= 16 ==> result == mk_u32 (pow2 (v y))}
-val overflowing_pow_u32 : u32 -> u32 -> u32 & bool
+val overflowing_pow_u32 : x:u32 -> y:u32 -> r:(u32 & bool) {snd r == not (range (int_pow (v x) (v y)) U32)}
 val count_ones_u32 : u32 -> r:u32{v r <= 32}
 
 let wrapping_add_u64 : u64 -> u64 -> u64 = add_mod
@@ -72,7 +75,7 @@ val saturating_mul_u64 : u64 -> u64 -> u64
 let overflowing_mul_u64 : u64 -> u64 -> u64 & bool = mul_overflow
 let rem_euclid_u64 (x: u64) (y: u64 {v y <> 0}): u64 = x %! y
 val pow_u64 : u64 -> u32 -> u64
-val overflowing_pow_u64 : u64 -> u32 -> u64 & bool
+val overflowing_pow_u64 : x:u64 -> y:u32 -> r:(u64 & bool) {snd r == not (range (int_pow (v x) (v y)) U64)}
 val count_ones_u64 : u64 -> r:u32{v r <= 64}
 
 let wrapping_add_u128 : u128 -> u128 -> u128 = add_mod
@@ -90,7 +93,7 @@ val saturating_mul_u128 : u128 -> u128 -> u128
 let overflowing_mul_u128 : u128 -> u128 -> u128 & bool = mul_overflow
 let rem_euclid_u128 (x: u128) (y: u128 {v y <> 0}): u128 = x %! y
 val pow_u128 : u128 -> u32 -> u128
-val overflowing_pow_u128 : u128 -> u32 -> u128 & bool
+val overflowing_pow_u128 : x:u128 -> y:u32 -> r:(u128 & bool) {snd r == not (range (int_pow (v x) (v y)) U128)}
 val count_ones_u128 : u128 -> r:u32{v r <= 128}
 
 let wrapping_add_usize : usize -> usize -> usize = add_mod
@@ -108,7 +111,7 @@ val saturating_mul_usize : usize -> usize -> usize
 let overflowing_mul_usize : usize -> usize -> usize & bool = mul_overflow
 let rem_euclid_usize (x: usize) (y: usize {v y <> 0}): usize = x %! y
 val pow_usize : usize -> u32 -> usize
-val overflowing_pow_usize : usize -> u32 -> usize & bool
+val overflowing_pow_usize : x:usize -> y:u32 -> r:(usize & bool) {snd r == not (range (int_pow (v x) (v y)) USIZE)}
 val count_ones_usize : usize -> r:u32{v r <= size_bits}
 
 let wrapping_add_i8 : i8 -> i8 -> i8 = add_mod
@@ -122,7 +125,7 @@ val saturating_mul_i8 : i8 -> i8 -> i8
 let overflowing_mul_i8 : i8 -> i8 -> i8 & bool = mul_overflow
 let rem_euclid_i8 (x: i8) (y: i8 {v y <> 0}): i8 = x %! y
 val pow_i8 : i8 -> u32 -> i8
-val overflowing_pow_i8 : i8 -> u32 -> i8 & bool
+val overflowing_pow_i8 : x:i8 -> y:u32 -> r:(i8 & bool) {snd r == not (range (int_pow (v x) (v y)) I8)}
 val count_ones_i8 : i8 -> r:u32{v r <= 8}
 /// `i8::abs`.  Rust documents the overflow case explicitly: "The absolute
 /// value of `i8::MIN` cannot be represented as an `i8`, and attempting to
@@ -146,7 +149,7 @@ val saturating_mul_i16 : i16 -> i16 -> i16
 let overflowing_mul_i16 : i16 -> i16 -> i16 & bool = mul_overflow
 let rem_euclid_i16 (x: i16) (y: i16 {v y <> 0}): i16 = x %! y
 val pow_i16 : x: i16 -> y:u32 -> result: i16 {v x == 2 /\ v y < 15 ==> (Math.Lemmas.pow2_lt_compat 15 (v y); result == mk_i16 (pow2 (v y)))}
-val overflowing_pow_i16 : i16 -> u32 -> i16 & bool
+val overflowing_pow_i16 : x:i16 -> y:u32 -> r:(i16 & bool) {snd r == not (range (int_pow (v x) (v y)) I16)}
 val count_ones_i16 : i16 -> r:u32{v r <= 16}
 /// `i16::abs`.  Rust documents the overflow case explicitly: "The absolute
 /// value of `i16::MIN` cannot be represented as an `i16`, and attempting to
@@ -170,7 +173,7 @@ val saturating_mul_i32 : i32 -> i32 -> i32
 let overflowing_mul_i32 : i32 -> i32 -> i32 & bool = mul_overflow
 let rem_euclid_i32 (x: i32) (y: i32 {v y <> 0}): i32 = x %! y
 val pow_i32 : x : i32 -> y:u32 -> result: i32 {v x == 2 /\ v y <= 16 ==> result == mk_i32 (pow2 (v y))}
-val overflowing_pow_i32 : i32 -> u32 -> i32 & bool
+val overflowing_pow_i32 : x:i32 -> y:u32 -> r:(i32 & bool) {snd r == not (range (int_pow (v x) (v y)) I32)}
 val count_ones_i32 : i32 -> r:u32{v r <= 32}
 /// `i32::abs`.  Rust documents the overflow case explicitly: "The absolute
 /// value of `i32::MIN` cannot be represented as an `i32`, and attempting to
@@ -194,7 +197,7 @@ val saturating_mul_i64 : i64 -> i64 -> i64
 let overflowing_mul_i64 : i64 -> i64 -> i64 & bool = mul_overflow
 let rem_euclid_i64 (x: i64) (y: i64 {v y <> 0}): i64 = x %! y
 val pow_i64 : i64 -> u32 -> i64
-val overflowing_pow_i64 : i64 -> u32 -> i64 & bool
+val overflowing_pow_i64 : x:i64 -> y:u32 -> r:(i64 & bool) {snd r == not (range (int_pow (v x) (v y)) I64)}
 val count_ones_i64 : i64 -> r:u32{v r <= 64}
 /// `i64::abs`.  Rust documents the overflow case explicitly: "The absolute
 /// value of `i64::MIN` cannot be represented as an `i64`, and attempting to
@@ -218,7 +221,7 @@ val saturating_mul_i128 : i128 -> i128 -> i128
 let overflowing_mul_i128 : i128 -> i128 -> i128 & bool = mul_overflow
 let rem_euclid_i128 (x: i128) (y: i128 {v y <> 0}): i128 = x %! y
 val pow_i128 : i128 -> u32 -> i128
-val overflowing_pow_i128 : i128 -> u32 -> i128 & bool
+val overflowing_pow_i128 : x:i128 -> y:u32 -> r:(i128 & bool) {snd r == not (range (int_pow (v x) (v y)) I128)}
 val count_ones_i128 : i128 -> r:u32{v r <= 128}
 /// `i128::abs`.  Rust documents the overflow case explicitly: "The absolute
 /// value of `i128::MIN` cannot be represented as an `i128`, and attempting to
@@ -242,7 +245,7 @@ val saturating_mul_isize : isize -> isize -> isize
 let overflowing_mul_isize : isize -> isize -> isize & bool = mul_overflow
 let rem_euclid_isize (x: isize) (y: isize {v y <> 0}): isize = x %! y
 val pow_isize : isize -> u32 -> isize
-val overflowing_pow_isize : isize -> u32 -> isize & bool
+val overflowing_pow_isize : x:isize -> y:u32 -> r:(isize & bool) {snd r == not (range (int_pow (v x) (v y)) ISIZE)}
 val count_ones_isize : isize -> r:u32{v r <= size_bits}
 /// `isize::abs`.  Rust documents the overflow case explicitly: "The absolute
 /// value of `isize::MIN` cannot be represented as an `isize`, and attempting to
